Added templates for methods to implement and defined Valid function

proj/TreeSet.dfy
@@ -1,59 +1,127 @@
-// A datatype that stores a value of type T or Nil (no value) 
-datatype Option<T> = Nil | Some(value: T)
-
 // Function type for comparing elements
-type ComparatorFunction<!T> = (T) -> nat 
+// TODO: depois ver se consigo por tipo generico mesmo
+type T = int // for demo purposes, but could be real, etc.
 
-// Represents a sorted set of elements of type T. 
-class {:autocontracts} TreeSet<T(==)> {
+// **********************************************************************
+// Represents a binary search tree node, for elements of type T.
 
-  // Abstract state variable used for specification purposes only (set of elements in the sorted set).  
+class BTNode {
+  var value: T; // value of the node
+  var left: BTNode?;  // left child of the node (? - may be null)
+  var right: BTNode?; // right child of the node (? - may be null)
+
+  // Constructor of the class.
+  constructor (value: T, left: BTNode?, right: BTNode?) 
+    ensures this.value == value
+    ensures this.left == left
+    ensures this.right == right
+  {
+    this.value := value;
+    this.left := left;
+    this.right := right;
+  }
+}
+
+// **********************************************************************
+// Represents a sorted set of elements of type T.
+
+// TODO: depois, ver se devia fazer com que bst fosse balanced (prob nao)
+// TODO: como ter a certeza que não há duplicados?
+class {:autocontracts} TreeSet {
+  // Ghost variable used for specification & verification purposes.
+  // Holds the set of values in the subtree starting in this node (inclusive). 
   ghost var elems : set<T>;
-
-   // Comparator function that it is passed to the tree set, so it can order its elements. 
-  const comp_func: ComparatorFunction<T>;
-
-  const initializer: nat -> T; // required by new T[]
-
+  
   // Concrete state variable with internal representation (initially filled with Nil). 
-  // TODO: ver representacao de uma BST
+  var root: BTNode?;
 
+  // Predicate that formalizes the class invariant. Makes sure that the binary tree starting at
+  // root is sorted (it is a binary search tree), and connects the abstract state variable (elems)
+  // to the actual set of elements in the binary tree, using the BTtoSet() function.
+  predicate Valid()
+  {
+    isBST(root) &&
+    elems == BSTtoSet(root)
+  }
 
-  // Predicate that formalizes the class invariant.
-  predicate Valid() { 
-    true
-    // TODO: class invariant
+  // Predicate that indicates if the binary tree is correctly sorted, and is a valid BST.
+  predicate isBST(node : BTNode?)
+    reads root
+    decreases elems
+  {
+    if node == null
+    then true
+    else (node.left != null ==> forall k :: k in BSTtoSet(node.left) ==> k < node.value) && 
+         (node.right != null ==> forall k :: k in BSTtoSet(node.right) ==> k > node.value) &&
+         isBST(node.left) && isBST(node.right)
+  }
+
+  function BSTtoSet(node : BTNode?) : set<T>
+    decreases node
+  {
+    if node == null
+    then {}
+    else {node.value} + BSTtoSet(node.left) + BSTtoSet(node.right)
   }
 
   // Receives the hash function to be used and initializes the set as empty.
-  constructor (comp_func: ComparatorFunction<T>) 
+  constructor () 
     ensures elems == {}
-    ensures this.comp_func == comp_func
   {
-    this.comp_func := comp_func;
+    this.root := null;
+    this.elems := {};
   }
 
   // Inserts a new element x into the sorted set (binary search tree).
-  method insert(x : T) {
+  method insert(x : T) 
+    requires x !in elems
+    ensures elems == old(elems) + {x}
+  {
+    root := this.insertAux(x, root);
+    this.elems := this.elems + {x};
+  }
 
+  method insertAux(x : T, node : BTNode?) returns (res : BTNode?)
+  {
+    // TODO: insert method
   }
 
   // Deletes an element X from the sorted set (binary search tree).
-  method delete(x : T) {
-
+  method delete(x : T) 
+    requires x in elems
+    ensures elems == old(elems) - {x}
+  {
+    root := this.deleteAux(x, root);
+    elems := elems - {x};
   }
 
+  method deleteAux(x : T, node : BTNode?) returns (res : BTNode?)
+  {
+    // TODO: delete method
+  }
 
-  // Checks if an element X is in the sorted set (binary search tree).
+  // Check if the subtree starting in this node contains a value 'x'.
   method contains(x: T) returns (res: bool)
+    ensures res <==> x in elems
   {
-
+    res := this.containsAux(x, root);
   }
 
-  // Returns an ordered sequence with all the elements of the sorted set (binary search tree).
-  method asSeq() returns (res: seq<T>)
+  method containsAux(x: T, node: BTNode?) returns (res: bool)
+    ensures res <==> x in BSTtoSet(node)
   {
+    // TODO: contains method
+  }
 
+  // Returns an ordered sequence with all the elements of the BST.
+  // Need to do an inorder traversal of the tree (left subtree first, then root, then right subtree).
+  method asSeq() returns (res : seq<T>)
+    ensures multiset(res) == multiset(elems)
+    ensures forall k1, k2 :: 0 <= k1 < k2 < |res| ==> res[k1] < res[k2]
+    decreases elems
+  {
+    // TODO: talvez seja preciso lemma para provar que subtree da esquerda é menor e a da direita é maior?
+    // TODO: asSeq method
   }
 }
 
